# Pr√°ctica 3 / Ejercicio 1

$v(P) = v(Q) = V$ \
$v(S) = v(T) = F$

## I.

$(\neg P \lor Q) = (\neg V \lor V) = (F \lor V) = V$

## II.

$(P \lor (S \land T) \lor Q) = (V \lor (F \land F) \lor V) = V$

## III.

$\neg(Q \lor S) = \neg(V \lor F) = \neg V = F$

## IV.

$(\neg P \lor S) \iff (\neg P \land \neg S)$ \
$= (\neg V \lor F) \iff (\neg V \land \neg F)$ \
$= (F \lor F) \iff (F \land V)$ \
$= F \iff F$ \
$= V$

## V.

$((P \lor S) \land (T \lor Q))$ \
$= ((V \lor F) \land (F \lor V))$ \
$= (V \land V)$ \
$= V$

## VI.

$(((P \lor S) \land (T \lor Q)) \iff (P \lor (S \land T) \lor Q))$ \
$= (((V \lor F) \land (F \lor V)) \iff (V \lor (F \land F) \lor V))$ \
$= ((V \land V) \iff (V \lor F \lor V))$ \
$= (V \iff V)$ \
$= V$

## VII.

$(\neg Q \land \neg S) = (\neg V \land \neg F) = (F \land V) = F$
