# Práctica 2 / Ejercicio 1

## I.

```hs
intercambiar (x,y) = (y,x)
```

```
∀p :: (a,b). intercambiar (intercambiar p) = p
```

Por principio de extensionalidad para pares basta ver que:

```
∀p :: (a,b). ∃x :: a. ∃y :: b. p = (x,y).
intercambiar (intercambiar (x,y)) = (x,y)
```

```
intercambiar (intercambiar (x,y))
= intercambiar (y,x)                {def intercambiar}
= (x,y)                             {def intercambiar}
```

## II.

```hs
asociarI (x,(y,z)) = ((x,y),z)
asociarD ((x,y),z) = (x,(y,z))
```

```
∀p :: (a,(b,c)). asociarD (asociarI p) = p
```

Por principio de extensionalidad para pares basta ver que:

```
∀p :: (a,(b,c)). ∃x :: a. ∃w :: (b,c). p = (x,w).
asociarD (asociarI (x,w)) = (x,w)
```

Por principio de extensionalidad para pares basta ver que:

```
∀p :: (a,(b,c)).
∃x :: a. ∃w :: (b,c). p = (x,w).
∃y :: b. ∃z :: c. w = (y,z). p = (x,(y,z)).
asociarD (asociarI (x,(y,z))) = (x,(y,z))
```

```
asociarD (asociarI (x,(y,z)))
= asociarD ((x,y),z)            {def asociarI}
= (x,(y,z))                     {def asociarD}
```

## III.

```hs
espejar (Left x) = Right x
espejar (Right x) = Left x
```

```
∀p :: Either a b. espejar (espejar p) = p
```

Por principio de extensionalidad para sumas basta ver que:

```
∀p :: Either a b
o bien ∃x :: a. p = Left x
o bien ∃y :: b. p = Right y
espejar (espejar p) = p
```

Caso `p = Left x`:

```
espejar (espejar (Left x))
= espejar (Right x)             {def espejar}
= Left x                        {def espejar}
```

Caso `p = Right x`:

```
espejar (espejar (Right x))
= espejar (Left x)              {def espejar}
= Right x                       {def espejar}
```

## IV.

```hs
flip f x y = f y x
```

```
∀f :: a -> b -> c. ∀x :: a. ∀y :: b. flip (flip f) x y = f x y
```

```
flip (flip f) x y
= (flip f) y x      {def flip}
= flip f y x        {asocia a izquierda}
= f x y             {def flip}
```

## V.

```hs
curry f x y = f (x,y)
uncurry f (x,y) = f x y
```

```
∀f :: a -> b -> c. ∀x :: a. ∀y :: b. curry (uncurry f) x y = f x y
```

```
curry (uncurry f) x y
= uncurry f (x,y)       {def curry}
= f x y                 {def uncurry}
```
